Recall Eqs. (6):

$$
a'm+b'n=c,\qquad am+bn=d.
$$

Recall also that step E4 sets $c\leftarrow d$, $d\leftarrow r$, $t\leftarrow a'$, $a'\leftarrow a$, $a\leftarrow t-qa$, $t\leftarrow b'$, $b'\leftarrow b$, $b\leftarrow t-qb$.

Assume that Eqs. (6) holds before step E4. If we prove that the equations

$$
am+bn=d,\qquad (a'-qa)m+(b'-qb)n=r
$$

hold, then the proof is complete because after step E4 these are equivalent to Eqs. (6).

And indeed these equations hold, because the first one the same as the second equation in (6), and the second one is implid from (6) and step E2 as follows:

$$
(a'-qa)m+(b'-qb)n = (a'm+b'n)-q(am+bn) = c - qd = r.
$$
