> Prove by induction that if $0\le a\le 1$, then $(1-a)^n\ge1-na$.

---

Base case: $n=1$.

$$
    (1-a)^n=(1-a)^1=1-a=1-1\cdot a=1-na.
$$

Induction step: Assume

$$
    (1-a)^n\ge1-na.
$$

Since $0<a<1$, we have $1-a>0$, so we can multiply both sides of the inequality by $1-a$ without changing the sign.

$$
\begin{align}
    (1-a)^{n+1}=(1-a)^n(1-a)\\
    \ge(1-na)(1-a)\\
    =1-a-na+na^2\\
    =1-(n+1)a+na^2.
\end{align}
$$

Because $n\ge1$ and $a^2>0$ we have $na^2\ge0$. Hence

$$
    1-(n+1)a+na^2\ge 1-(n+1)a,
$$

so

$$
    (1-a)^{n+1}\ge1-(n+1)a,
$$

which concludes the proof.
